specs/tests/Spec.HPKE.Test.fst
@@ -12,6 +12,9 @@ module HPKE = Spec.Agile.HPKE
 module DH = Spec.Agile.DH
 module AEAD = Spec.Agile.AEAD
 module Hash = Spec.Agile.Hash
+module HKDF = Spec.Agile.HKDF
+
+friend Spec.Agile.HPKE
 
 // Test1: A.1, DHKEM(Curve25519), HKDF-SHA256, AES-GCM-128
 // Base Setup
@@ -477,16 +480,92 @@ let test_base_setup
   (skR:list uint8{List.Tot.length skR == HPKE.size_dh_key cs})
   (skI:list uint8{List.Tot.length skI == HPKE.size_dh_key cs})
   (skE:list uint8{List.Tot.length skE == HPKE.size_dh_key cs})
-  (psk pskID:list uint8)
+  (psk:list uint8) // {List.Tot.length psk == HPKE.size_psk cs})
+  (pskID:list uint8) //{List.Tot.length pskID <= HPKE.max_pskID})
   (pkR:list uint8{List.Tot.length pkR == HPKE.size_dh_public cs})
   (pkI:list uint8{List.Tot.length pkI == HPKE.size_dh_public cs})
   (pkE:list uint8{List.Tot.length pkE == HPKE.size_dh_public cs})
   (enc:list uint8)
   (zz:list uint8{List.Tot.length zz == HPKE.size_dh_public cs})
-  (context secret:list uint8)
+  (context:list uint8) //{List.Tot.length context == 9 + 3 * HPKE.size_dh_public cs + 2 * Hash.size_hash (HPKE.hash_of_cs cs)})
+  (secret:list uint8)
   (key:list uint8{List.Tot.length key == HPKE.size_aead_key cs})
   (nonce:list uint8{List.Tot.length nonce == HPKE.size_aead_nonce cs})
-= IO.print_string "Test setupBaseI\n";
+= IO.print_string "Test encap\n";
+  let encap = HPKE.encap cs (of_list skE) (of_list pkR) in
+  let res_encap =
+    if None? encap then (
+       IO.print_string "encap returned None\n"; false
+    ) else (
+      let (returned_zz, returned_pkE) = Some?.v encap in
+      let r2_a = for_all2 (fun a b -> uint_to_nat #U8 a = uint_to_nat #U8 b)
+        (of_list pkE) returned_pkE in
+      let r2_b = for_all2 (fun a b -> uint_to_nat #U8 a = uint_to_nat #U8 b)
+        (of_list zz) returned_zz in
+      if not r2_a then (
+        IO.print_string "\nExpected pkE :";
+        List.iter (fun a -> IO.print_string (UInt8.to_string (u8_to_UInt8 a))) pkE;
+        IO.print_string "\nComputed pkE :";
+        List.iter (fun a -> IO.print_string (UInt8.to_string (u8_to_UInt8 a))) (to_list returned_pkE);
+        IO.print_string "\n");
+      if not r2_b then (
+        IO.print_string "\nExpected zz :";
+        List.iter (fun a -> IO.print_string (UInt8.to_string (u8_to_UInt8 a))) zz;
+        IO.print_string "\nComputed zz :";
+        List.iter (fun a -> IO.print_string (UInt8.to_string (u8_to_UInt8 a))) (to_list returned_zz);
+        IO.print_string "\n");
+      r2_a && r2_b
+    )
+
+  in
+
+  IO.print_string "Test ks_derive\n";
+
+  let (psk, pskID) = (HPKE.default_psk cs, HPKE.default_pskId) in
+  let pkI = HPKE.default_pkI cs in
+  let pskID_hash = Hash.hash (HPKE.hash_of_cs cs) pskID in
+  let info_hash = Hash.hash (HPKE.hash_of_cs cs) (of_list info) in
+  let returned_context = HPKE.build_context HPKE.Base cs (of_list pkE) (of_list pkR) pkI pskID_hash info_hash in
+
+
+  IO.print_string "\nExpected context :";
+  List.iter (fun a -> IO.print_string (UInt8.to_string (u8_to_UInt8 a))) context;
+  IO.print_string "\nComputed context :";
+  List.iter (fun a -> IO.print_string (UInt8.to_string (u8_to_UInt8 a))) (to_list returned_context);
+  IO.print_string "\n";
+
+  let returned_secret = HKDF.extract (HPKE.hash_of_cs cs) psk (of_list zz) in
+
+  IO.print_string "\nExpected secret :";
+  List.iter (fun a -> IO.print_string (UInt8.to_string (u8_to_UInt8 a))) secret;
+  IO.print_string "\nComputed secret :";
+  List.iter (fun a -> IO.print_string (UInt8.to_string (u8_to_UInt8 a))) (to_list returned_secret);
+  IO.print_string "\n";
+
+
+  let info_key = Seq.append HPKE.label_key (of_list context) in
+  let info_nonce = Seq.append HPKE.label_nonce (of_list context) in
+  let keyIR = HKDF.expand (HPKE.hash_of_cs cs) returned_secret info_key (HPKE.size_aead_key cs) in
+  let nonceIR = HKDF.expand (HPKE.hash_of_cs cs) returned_secret info_nonce (HPKE.size_aead_nonce cs) in
+
+  IO.print_string "\nExpected key :";
+  List.iter (fun a -> IO.print_string (UInt8.to_string (u8_to_UInt8 a))) key;
+  IO.print_string "\nComputed key :";
+  List.iter (fun a -> IO.print_string (UInt8.to_string (u8_to_UInt8 a))) (to_list keyIR);
+  IO.print_string "\n";
+
+  IO.print_string "\nExpected nonce :";
+  List.iter (fun a -> IO.print_string (UInt8.to_string (u8_to_UInt8 a))) nonce;
+  IO.print_string "\nComputed nonce :";
+  List.iter (fun a -> IO.print_string (UInt8.to_string (u8_to_UInt8 a))) (to_list nonceIR);
+  IO.print_string "\n";
+
+
+
+  // let k, n = HPKE.ks_derive cs HPKE.Base (of_list pkR) (of_list zz) (of_list pkE)
+  //   (of_list info) None None in
+
+  IO.print_string "Test setupBaseI\n";
   let setupBaseI = HPKE.setupBaseI cs (of_list skE) (of_list pkR) (of_list info) in
   let res_setupBaseI =
     if None? setupBaseI then (
@@ -540,10 +619,13 @@ let test () =
   assert_norm (List.Tot.length test1_skR == HPKE.size_dh_key cs1);
   assert_norm (List.Tot.length test1_skI == HPKE.size_dh_key cs1);
   assert_norm (List.Tot.length test1_skE == HPKE.size_dh_key cs1);
+  assert_norm (List.Tot.length test1_pskID <= HPKE.max_pskID);
   assert_norm (List.Tot.length test1_pkR == HPKE.size_dh_public cs1);
   assert_norm (List.Tot.length test1_pkI == HPKE.size_dh_public cs1);
   assert_norm (List.Tot.length test1_pkE == HPKE.size_dh_public cs1);
   assert_norm (List.Tot.length test1_zz == HPKE.size_dh_public cs1);
+  // assert_norm (List.Tot.length test1_context == 9 + 3 * HPKE.size_dh_public cs1 + 2 * Hash.size_hash (HPKE.hash_of_cs cs1));
+
   assert_norm (List.Tot.length test1_key == HPKE.size_aead_key cs1);
   assert_norm (List.Tot.length test1_nonce == HPKE.size_aead_nonce cs1);
 
